work on repl stuff in Unfold, add relEquiv

Pdl/Unfold.lean
@@ -1,6 +1,7 @@
 -- UNFOLD
 
 import Pdl.Semantics
+import Pdl.Vocab
 
 -- TODO: move to Syntax.lean
 mutual
@@ -8,7 +9,7 @@ mutual
   def repl_in_F (x : Char) (ψ : Formula) : Formula → Formula
     | ⊥ => ⊥
     | ·c => if c == x then ψ else ·c
-    | ~φ => (repl_in_F x ψ) φ
+    | ~φ => ~(repl_in_F x ψ φ)
     | φ1⋀φ2 => (repl_in_F x ψ) φ1 ⋀ (repl_in_F x ψ) φ2
     | ⌈α⌉ φ => ⌈repl_in_P x ψ α⌉ (repl_in_F x ψ φ)
   @[simp]
@@ -20,11 +21,56 @@ mutual
     | ?'φ  => ?' (repl_in_F x ψ φ)
 end
 
-theorem repl_in_F_equiv x ψ:
-    (φ1 ≡ φ2) → (repl_in_F x ψ φ1) ≡ (repl_in_F x ψ φ2) := by sorry
+open HasVocabulary
+
+mutual
+theorem repl_in_F_non_occ_eq {x φ ρ} :
+    x ∉ voc φ → repl_in_F x ρ φ = φ := by
+  intro x_notin_phi
+  cases φ
+  case bottom => simp
+  case atom_prop c =>
+    simp only [repl_in_F, beq_iff_eq, ite_eq_right_iff]
+    intro c_is_x; simp [voc,vocabOfFormula] at *; tauto
+  case neg φ0 =>
+    simp [voc,vocabOfFormula] at *
+    apply repl_in_F_non_occ_eq; tauto
+  case and φ1 φ2 =>
+    simp [voc,vocabOfFormula] at *
+    constructor <;> (apply repl_in_F_non_occ_eq ; tauto)
+  case box α φ0 =>
+    simp [voc,vocabOfFormula] at *
+    constructor
+    · apply repl_in_P_non_occ_eq; tauto
+    · apply repl_in_F_non_occ_eq; tauto
+theorem repl_in_P_non_occ_eq {x α ρ} :
+    x ∉ voc α → repl_in_P x ρ α = α := by
+  intro x_notin_alpha
+  cases α
+  all_goals simp [voc,vocabOfProgram] at *
+  case sequence β γ =>
+    constructor <;> (apply repl_in_P_non_occ_eq; tauto)
+  case union β γ =>
+    constructor <;> (apply repl_in_P_non_occ_eq; tauto)
+  case star β =>
+    apply repl_in_P_non_occ_eq ; tauto
+  case test φ =>
+    apply repl_in_F_non_occ_eq; tauto
+end
+
+-- TODO: move to Semantics?
+
+mutual
+theorem repl_in_F_equiv x ψ :
+    (φ1 ≡ φ2) → (repl_in_F x ψ φ1) ≡ (repl_in_F x ψ φ2) := sorry
+
+theorem repl_in_P_equiv x ψ :
+    (α1 ≡ᵣ α2) → (repl_in_P x ψ α1) ≡ᵣ (repl_in_P x ψ α2) := sorry
+end
 
 -- Lemma 45 from Yde
 theorem fortyfive (x : Char)
+    (x_notin_beta : x ∉ HasVocabulary.voc β)
     (beta_equiv : (⌈β⌉·x) ≡ (((·x) ⋀ χ0) ⋁ χ1))
     (rho_imp_repl : ρ ⊨ (repl_in_F x ρ) (χ0 ⋁ χ1))
     (rho_imp_psi : ρ ⊨ ψ)
@@ -41,13 +87,11 @@ theorem fortyfive (x : Char)
         tauto
       -- Now we want to "rewrite" with beta_equiv.
       have := repl_in_F_equiv x ρ beta_equiv
-      simp at this
-      -- Do we need that x ∉ β ???
-      have nox : repl_in_P x ρ β = β := sorry
+      simp only [repl_in_F, beq_self_eq_true, reduceIte, Formula.or] at this
+      have nox : repl_in_P x ρ β = β := repl_in_P_non_occ_eq x_notin_beta
       rw [nox] at this
       rw [equiv_iff this]
-      simp [evaluate,relate,modelCanSemImplyForm] at *
-      tauto
+      simp_all
     -- It is then immediate...
     simp [evaluate,relate,modelCanSemImplyForm] at this
     exact this v w_β_v -- This finishes the proof of (46).
@@ -57,6 +101,6 @@ theorem fortyfive (x : Char)
   intro w_rho v w_bS_v
   induction w_bS_v using Relation.ReflTransGen.head_induction_on
   · apply rho_imp_psi; simp; assumption; simp
-  case head u1 u2 u1_b_u2 u1_bS_u2 IH =>
+  case head u1 u2 u1_b_u2 _ IH =>
     apply IH
     exact fortysix W M u1 u2 w_rho u1_b_u2
